src/Lib/DWTVSTSpec.v
@@ -1,0 +1,59 @@
+Require Import Core.Core Core.StructNormalizer VstLib DWTExecSpec ErrorWithWriter.
+Require Import VST.floyd.proofauto Psatz.
+Require Import Clight.der_encoder.
+
+Definition Vprog : varspecs. mk_varspecs prog. Defined.
+Instance CompSpecs : compspecs. make_compspecs prog. Defined.
+
+Open Scope Z.
+
+Section Der_write_tags.
+
+Definition der_write_tags_spec : ident * funspec :=
+  DECLARE _der_write_tags
+    WITH (* pointer to type descriptor structure *) 
+         sd_b : block, sd_ofs : ptrofs, sd : TYPE_descriptor, sh_sd : share,
+         struct_l : Z, tag_mode : Z, last_tag_form : Z, tag : Z,
+         (* callback pointer *)
+         cb_b : block, cb_ofs : ptrofs, cb_val : val, sh_cb : share,
+         (* callback argument pointer *)
+         app_key_b : block, app_key_ofs : ptrofs,
+         app_key_val : val, sh_app_key : share
+    PRE [ _sd OF (tptr (Tstruct _asn_TYPE_descriptor_s noattr)),
+          _struct_length OF tuint, _tag_mode OF tint,
+          _last_tag_form OF tint, _tag OF tuint,
+          _cb OF cb_type, _app_key OF (tptr tvoid) ]
+    PROP ( readable_share sh_sd;
+           readable_share sh_cb;
+           readable_share sh_app_key )
+    LOCAL ( temp _sd (Vptr sd_b sd_ofs);
+            temp _struct_length (Vint (Int.repr struct_l));
+            temp _tag_mode (Vint (Int.repr tag_mode));
+            temp _last_tag_form (Vint (Int.repr last_tag_form));
+            temp _tag (Vint (Int.repr tag));
+            temp _cb (Vptr cb_b cb_ofs);
+            temp _app_key (Vptr app_key_b app_key_ofs))
+    SEP ( data_at sh_sd (Tstruct _asn_TYPE_descriptor_s noattr) 
+                  (TYPE_descriptor_rep sd) (Vptr sd_b sd_ofs) ; 
+          data_at sh_app_key (tvoid) (tt) (Vptr app_key_b app_key_ofs) ;
+          data_at sh_cb (cb_type) (tt) (Vptr cb_b cb_ofs))
+    POST [tint]
+      PROP ()
+      LOCAL (temp ret_temp (Vint (Int.repr (
+                                      match evalErrW (der_write_tags sd) [] with
+                                      | Some w => encoded w
+                                      | None => -1
+                                      end))))
+      SEP ( (* Unchanged by the execution : *)
+            data_at sh_sd (Tstruct _asn_TYPE_descriptor_s noattr) 
+                    (TYPE_descriptor_rep sd) (Vptr sd_b sd_ofs) ; 
+            data_at sh_app_key (tvoid) (tt) 
+                    (Vptr app_key_b app_key_ofs) ;
+            data_at sh_cb (cb_type) (tt) (Vptr cb_b cb_ofs)).
+
+Definition Gprog := ltac:(with_library prog [der_write_tags_spec]).
+
+Theorem bool_der_encode : semax_body Vprog Gprog (normalize_function f_der_write_tags composites) der_write_tags_spec.
+Admitted.
+
+End Der_write_tags.
